# 続き - 解答

### (2)
[cite_start]$F(x,y,\lambda) = xy-\lambda(x^{3}+y^{3}+x+y-4)$ [cite: 205]
[cite_start]$F_{x}=F_{y}=F_{\lambda}=0$ を解く [cite: 206]
[cite_start]$F_{x}=y-3\lambda x^{2}-\lambda, F_{y}=x-3\lambda y^{2}-\lambda, F_{\lambda}=-x^{3}-y^{3}-x-y+4$ [cite: 207]
[cite_start]$$egin{cases} y=\lambda(3x^{2}+1) \ x=\lambda(3y^{2}+1) \ x^{3}+y^{3}+x+y-4=0 \end{cases}$$ [cite: 208]
[cite_start]$\lambda = rac{y}{3x^{2}+1} = rac{x}{3y^{2}+1}$ [cite: 210]
[cite_start]$y(3y^{2}+1)=x(3x^{2}+1)$ [cite: 209]
[cite_start]$3y^{3}+y=3x^{3}+x \implies 3(x^{3}-y^{3})+(x-y)=0$ [cite: 210]
[cite_start]$3(x-y)(x^{2}+xy+y^{2})+(x-y)=0$ [cite: 210]
[cite_start]$(x-y)\{3(x^{2}+xy+y^{2})+1\}=0$ [cite: 210]
[cite_start]$3(x^{2}+xy+y^{2})+1 > 0$ なので $x-y=0 \implies x=y$ [cite: 211]
[cite_start]制約条件に代入: $x^{3}+x^{3}+x+x-4=0 \implies 2x^{3}+2x-4=0 \implies 2(x^{3}+x-2)=0$ [cite: 212]
[cite_start]$2(x-1)(x^{2}+x+2)=0$ [cite: 213]
$x^{2}+x+2 = (x+rac{1}{2})^{2}+rac{7}{4} > 0$
[cite_start]よって $x=1$ [cite: 215]
[cite_start]$x=y=1$ より $(x,y)=(1,1)$ [cite: 215]
[cite_start]$f(1,1)=1\cdot 1=1$ [cite: 214]
[cite_start]$x	o\infty$ のとき、制約条件 $x^{3}+y^{3}+x+y-4=0$ を満たすためには、$y	o -\infty$ でなくてはいけない。 [cite: 216]
[cite_start]そしてそのとき $f(x,y)=xy 	o -\infty$ [cite: 217]
[cite_start]同様に $x	o -\infty$ のときは $y	o \infty$ で $f(x,y) 	o -\infty$ [cite: 217, 218]
[cite_start]よって、$(x,y)=(1,1)$ のとき最大値1、最小値なし [cite: 219]