# 続き - 解答

[cite_start]$F(x,y,\lambda) = f(x,y)-\lambda \phi(x,y) = 2xy-\lambda(x^{3}+y^{3}+2x+2y-6)$ [cite: 281, 282]
[cite_start]$F_{x}=F_{y}=F_{\lambda}=0$ を解く [cite: 283]
[cite_start]$F_{x}=2y-3\lambda x^{2}-2\lambda, F_{y}=2x-3\lambda y^{2}-2\lambda$ [cite: 284]
[cite_start]$F_{x}-F_{y}=0 \implies 2y-2x-3\lambda x^{2}+3\lambda y^{2}=0$ [cite: 285]
$2(y-x)-3\lambda(x^{2}-y^{2})=0$
$2(y-x)+3\lambda(y-x)(x+y)=0$
[cite_start]$(y-x)\{2+3\lambda(x+y)\}=0$ [cite: 288]
$x=y$ または $2+3\lambda(x+y)=0$

1. [cite_start]$x=y$ のとき [cite: 294]
[cite_start]制約条件に代入: $x^{3}+x^{3}+2x+2x-6=0 \implies 2x^{3}+4x-6=0$ [cite: 289, 290]
[cite_start]$2(x^{3}+2x-3)=0 \implies 2(x-1)(x^{2}+x+3)=0$ [cite: 291]
[cite_start]$x^{2}+x+3>0$ より $x=1$ [cite: 292]
[cite_start]極値候補は $(1,1)$, $f(1,1)=2(1)(1)=2$ [cite: 293]

2. $2+3\lambda(x+y)=0$ のとき $\lambda = -rac{2}{3(x+y)}$
$\lambda$ を $F_{x}=0$ に代入: $2y-3(-rac{2}{3(x+y)})x^{2}-2(-rac{2}{3(x+y)})=0$
$2y+rac{2x^{2}}{x+y}+rac{4}{3(x+y)}=0 \implies 6y(x+y)+6x^{2}+4=0 \implies 6xy+6y^{2}+6x^{2}+4=0$
$6(x^{2}+xy+y^{2})+4=0$
$x^{2}+xy+y^{2} \ge rac{1}{4}(x+y)^{2} + rac{3}{4}(x-y)^{2} \ge 0$ なので、これは解なし

[cite_start]$x	o\infty$ ならば $\phi=0$ を満たすには $y	o -\infty$ が必要 [cite: 295]
[cite_start]このとき $f(x,y)=2xy 	o -\infty$ [cite: 296]
[cite_start]$f(1,1)=2$ は最大値、最小値なし [cite: 297]