# 続き - 解答

[cite_start]$(\chi,y) \mapsto (t,s)=(2x+y, x-y) \mapsto f(t(x,y), s(x,y))$ ($f$ : 微分可)とする。 [cite: 313]
(1) [cite_start]$f_{x}, f_{y}$ を $f_{t}, f_{s}$ で表せ [cite: 314]
(2) [cite_start]$f_{t}, f_{s}$ を $f_{x}, f_{y}$ で表せ [cite: 315]

[cite_start]$$egin{cases} t=2x+y \ s=x-y \end{cases}$$ [cite: 316]

### (1)
[cite_start]$$rac{\partial f}{\partial x} = rac{\partial f}{\partial t}rac{\partial t}{\partial x} + rac{\partial f}{\partial s}rac{\partial s}{\partial x} = f_{t}\cdot 2 + f_{s}\cdot 1 = 2f_{t}+f_{s}$$ [cite: 318, 323]
[cite_start]$$rac{\partial f}{\partial y} = rac{\partial f}{\partial t}rac{\partial t}{\partial y} + rac{\partial f}{\partial s}rac{\partial s}{\partial y} = f_{t}\cdot 1 + f_{s}\cdot (-1) = f_{t}-f_{s}$$ [cite: 319, 320]

### (2)
[cite_start]$t+s = (2x+y)+(x-y)=3x \implies x = rac{1}{3}t+rac{1}{3}s$ [cite: 324]
[cite_start]$t-2s = (2x+y)-2(x-y)=3y \implies y = rac{1}{3}t-rac{2}{3}s$ [cite: 322]
[cite_start]$$rac{\partial f}{\partial t} = rac{\partial f}{\partial x}rac{\partial x}{\partial t} + rac{\partial f}{\partial y}rac{\partial y}{\partial t} = f_{x}\cdot rac{1}{3} + f_{y}\cdot rac{1}{3} = rac{1}{3}f_{x}+rac{1}{3}f_{y}$$ [cite: 326, 327]
[cite_start]$$rac{\partial f}{\partial s} = rac{\partial f}{\partial x}rac{\partial x}{\partial s} + rac{\partial f}{\partial y}rac{\partial y}{\partial s} = f_{x}\cdot rac{1}{3} + f_{y}\cdot (-rac{2}{3}) = rac{1}{3}f_{x}-rac{2}{3}f_{y}$$ [cite: 326, 327]